src/Options.v
@@ -3,9 +3,11 @@
 Record options : Set :=
   mkOptions {
       add_carry_constraints : bool;
-      rewrite_assignments : bool
+      rewrite_assignments : bool;
+      vars_cache_in_rewrite_assignments : bool
     }.
 
 Definition default_options : options :=
   {| add_carry_constraints := false;
-     rewrite_assignments := true |}.
+     rewrite_assignments := true;
+     vars_cache_in_rewrite_assignments := true |}.
